Compatibility WIP (replacing capture-avoiding subst)

src/CIU.v
@@ -1,10 +1,58 @@
 Require Import LogRel.
 Import ListNotations.
 
+(* Inductive Frame : Set :=
+| FApp1 (l : list Exp) (* apply □(e₁, e₂, ..., eₙ) *)
+| FApp2 (v : Exp) (p : is_value v) (l1 l2 : list Exp) (p2 : forall e, In e l2 -> is_value e) (** Can be problematic *)
+| FLet (v : Var) (e2 : Exp) (* let v = □ in e2 *)
+| FPlus1 (e2 : Exp) (* □ + e2 *)
+| FPlus2 (v : Exp) (p : is_value v) (* v + □ *)
+| FIf (e2 e3 : Exp) (* if □ then e2 else e3 *).
+
+Definition merge (F : Frame) (e : Exp) :=
+match F with
+ | FApp1 l => 
+ | FApp2 v p l1 l2 p2 => _
+ | FLet v e2 => _
+ | FPlus1 e2 => _
+ | FPlus2 v p => _
+ | FIf e2 e3 => _
+end
+
+
+Definition FrameStack := list Frame.
+
+Inductive Configuration : Type :=
+| ConfigReady (e : Exp)
+| ConfigStep (e : Exp) (F : FrameStack).
+
+Definition step (c : Configuration) : option Configuration :=
+match c with
+| ConfigReady e => None (* Should not be this ID? *)
+| ConfigStep e F =>
+  match e with
+  | ELit l =>
+    match F with
+    | [] => ConfigReady (ELit l)
+    | f::fs => ConfigStep (merge f (ELit l)) fs
+    end
+  | EVar v => _
+  | EFunId f => _
+  | EFun vl e => _
+  | ERecFun f vl e => _
+  | EApp exp l => _
+  | ELet v e1 e2 => _
+  | ELetRec f vl b e => _
+  | EPlus e1 e2 => _
+  | EIf e1 e2 e3 => _
+  end
+end. *)
+
+
 Definition CIU (e1 e2 : Exp) : Prop :=
   EXPCLOSED e1 /\ EXPCLOSED e2 /\
-  forall v1 v2, CIU_equivalent_values v1 v2 ->
-  (exists clock, eval clock e1 = Res v1) <-> (exists clock, eval clock e2 = Res v2).
+  forall v1 clock,
+  eval clock e1 = Res v1 -> (exists v2, exists clock, eval clock e2 = Res v2 /\ equivalent_values v1 v2).
 
 Definition CIU_open (Γ : list VarFunId) (e1 e2 : Exp) :=
   forall ξ, subscoped Γ [] ξ ->
@@ -17,15 +65,71 @@ Proof.
   intros. unfold CIU in H. intuition.
 Qed.
 
+Lemma CIU_closed_l : forall {e1 e2},
+    CIU e1 e2 ->
+    EXPCLOSED e1.
+Proof.
+  intros.
+  apply CIU_closed in H.
+  intuition.
+Qed.
+
+Hint Resolve CIU_closed_l.
+
+Lemma CIU_closed_r : forall {e1 e2},
+    CIU e1 e2 ->
+    EXPCLOSED e2.
+Proof.
+  intros.
+  apply CIU_closed in H.
+  intuition.
+Qed.
+
+Hint Resolve CIU_closed_r.
+
+Lemma CIU_open_scope : forall {Γ e1 e2},
+    CIU_open Γ e1 e2 ->
+    EXP Γ ⊢ e1 /\ EXP Γ ⊢ e2.
+Proof.
+  intros.
+  unfold CIU_open in H.
+  split;
+    eapply sub_implies_scope_exp; eauto.
+Qed.
+
+Lemma CIU_open_scope_l : forall {Γ e1 e2},
+    CIU_open Γ e1 e2 ->
+    EXP Γ ⊢ e1.
+Proof.
+  intros.
+  apply CIU_open_scope in H.
+  intuition.
+Qed.
+
+Hint Resolve CIU_open_scope_l.
+
+Lemma CIU_open_scope_r : forall {Γ e1 e2},
+    CIU_open Γ e1 e2 ->
+    EXP Γ ⊢ e2.
+Proof.
+  intros.
+  apply CIU_open_scope in H.
+  intuition.
+Qed.
+
+
+Hint Resolve CIU_open_scope_r.
 
 Lemma Erel_implies_CIU : forall Γ e1 e2,
   Erel_open Γ e1 e2 ->
   CIU_open Γ e1 e2.
 Proof.
-  intros. unfold CIU_open, CIU; intros.
-  split. 2: split. 3: assert (EXPCLOSED (subst ξ e1) /\ EXPCLOSED (subst ξ e2)).
-  1-3: eapply Erel_open_closed in H; eauto; apply H.
-  intros. destruct H1. unfold Erel_open, Erel in H. unfold exp_rel in H.
-  split; intros; inversion H3.
-  - unfold CIU_equivalent_values in H2. destruct H2, H2.
+  intros.
+  unfold CIU_open; intros.
+  unfold CIU.
+  split; [|split].
+  - eapply subst_preserves_scope_rev; eauto.
+  - eapply subst_preserves_scope_rev; eauto.
+  - intros. unfold Erel_open, Erel, exp_rel in H.
+    (* Vrel reflexivity needed *)
 Qed.
