src/Compatibility.v
@@ -74,7 +74,7 @@ Proof.
       rewrite var_funid_eqb_refl. auto.
 Qed.
 
-Lemma subst_composition :
+(* Lemma subst_composition :
   forall e ξ l vals Γ, length l = length vals -> subscoped Γ [] ξ ->
   EXP Γ ++ l ⊢ e ->
   composition (subst (idsubst[[ ::= combine l vals]])) (subst (ξ -- l)) e = subst (ξ[[::= combine l vals]]) e.
@@ -94,7 +94,7 @@ Proof.
       specialize (H0 _ H3). eapply vclosed_ignores_sub in H0. rewrite H0. reflexivity.
   * assert ((subst ((idsubst [[ ::= combine l vals]]) -- map inl vl) (subst ((ξ -- l) -- map inl vl) e)) = (subst ((ξ [[ ::= combine l vals]]) -- map inl vl) e)).
     { unfold composition in IHe.
-Abort.
+Abort. *)
 
 Definition varname (e : Exp) : option VarFunId :=
 match e with
@@ -133,14 +133,14 @@ Proof.
       eapply app_not_in in Heqb; eauto. apply not_in_list_sound in Heqb. rewrite Heqb. auto.
 Qed.
 
-Lemma subst_composition :
+(* Lemma subst_composition :
   forall e ξ η l,
   (subst (η[[::= l]])) (subst (ξ -- fst (split l)) e) = 
   subst (substcomp (η[[::= l]]) (ξ -- fst (split l))) e.
 Proof.
   induction e; intros; auto; simpl.
   * Search "--". rewrite subst_restrict_app.
-Abort.
+Abort. *)
 
 (** In general, the following lemma could not be weakened more:
     (ξ₁ -- l) cannot be replaced by ξ₁ on the right-hand side.
@@ -169,6 +169,48 @@ Proof.
   eapply vclosed_ignores_sub in H. rewrite H. auto.
 Qed.
 
+(* Lemma subscoped_app_restrict : forall Γ ξ Γ' l,
+  subscoped Γ Γ' ξ -> subscoped (Γ ++ l) Γ' (ξ -- l).
+Proof.
+  intros. unfold subscoped in *. intros. unfold "--". break_match_goal.
+Abort. *)
+(* 
+Fixpoint bound_variables (e : Exp) : list VarFunId :=
+match e with
+ | ELit l => []
+ | EVar v => []
+ | EFunId f => []
+ | EFun vl e => map inl vl ++ bound_variables e
+ | ERecFun f vl e => inr f :: map inl vl ++ bound_variables e
+ | EApp exp l => bound_variables exp ++ fold_left (fun acc e => bound_variables e ++ acc) l []
+ | ELet v e1 e2 => inl v :: bound_variables e1 ++ bound_variables e2
+ | ELetRec f vl b e => inr f :: map inl vl ++ bound_variables b ++ bound_variables e
+ | EPlus e1 e2 => bound_variables e1 ++ bound_variables e2
+ | EIf e1 e2 e3 => bound_variables e1 ++ bound_variables e2 ++ bound_variables e3
+end.
+
+Fixpoint free_variables (e : Exp) : list VarFunId :=
+match e with
+ | ELit l => []
+ | EVar v => [inl v]
+ | EFunId f => [inr f]
+ | EFun vl e => filter (fun name => negb (in_list name (map inl vl))) (free_variables e)
+ | ERecFun f vl e => filter (fun name => negb (in_list name (inr f :: map inl vl))) (free_variables e)
+ | EApp exp l => free_variables exp ++ fold_left (fun acc e => free_variables e ++ acc) l []
+ | ELet v e1 e2 => free_variables e1 ++ filter (fun name => negb (var_funid_eqb name (inl v))) (free_variables e2)
+ | ELetRec f vl b e => filter (fun name => negb (in_list name (inr f :: map inl vl))) (free_variables b) ++ filter (fun name => negb (var_funid_eqb name (inr f))) (free_variables e)
+ | EPlus e1 e2 => free_variables e1 ++ free_variables e2
+ | EIf e1 e2 e3 => free_variables e1 ++ free_variables e2 ++ free_variables e3
+end.
+
+Compute free_variables (sum 114).
+
+Local Definition l1 := ELet "X"%string (EVar "X"%string) (EVar "X"%string).
+Compute bound_variables l1.
+
+Definition capture_avoiding_subst (l : list VarFunId) (ξ : Substitution) :=
+  forall x, filter (fun name => in_list name l) (free_variables (ξ x)) = []. *)
+
 Corollary substcomp_restrict_subscoped : forall e ξ₁ ξ₂ l Γ, subscoped Γ [] ξ₂ ->
   EXP Γ ⊢ e ->
   subst (substcomp (ξ₁ -- l) (ξ₂ -- l)) e = subst (substcomp ξ₁ ξ₂ -- l) e.
@@ -176,28 +218,35 @@ Proof.
   induction e; intros; simpl; auto.
   * apply substcomp_restrict_x. apply H. inversion H0. inversion H1. auto.
   * apply substcomp_restrict_x. apply H. inversion H0. inversion H1. auto.
-  *
+  * inversion H0. inversion H1. subst.
+    rewrite subst_restrict_comm. erewrite <- IHe.
+    rewrite subst_restrict_comm. replace ((ξ₂ -- l) -- map inl vl) with ((ξ₂ -- map inl vl) -- l). 2: apply subst_restrict_comm. repeat rewrite subst_restrict_app. erewrite IHe.
+    auto.
+  
+(* (*     rewrite subst_restrict_comm, substcomp_restrict, subst_restrict_comm. erewrite IHe. 3: eauto.
+    subst_restrict_comm. auto. *) *)
 Abort.
 
 (**
   with capture-avoiding substitution, this should be trivial
+
+  However, if we substitute bound variables to closed values, it should not be a problem.
 *)
 Lemma subst_composition2 :
-  forall e ξ₁ ξ₂ , (* Γ, subscoped Γ [] ξ₁ -> subscoped Γ [] ξ₂ ->
-  EXP Γ ⊢ e ->*)
+  forall e ξ₁ ξ₂ Γ, EXP Γ ⊢ e -> subscoped Γ [] ξ₂ ->
   (subst ξ₁) (subst ξ₂ e) = subst (substcomp ξ₁ ξ₂) e.
 Proof.
   induction e; intros; simpl; auto.
-  * erewrite IHe, substcomp_restrict.
-Abort.
+  * erewrite IHe.
+Admitted.
 
-Lemma subst_composition_scoped :
+(* Lemma subst_composition_scoped :
   forall ξ η Γ Γ', subscoped Γ Γ' ξ -> subscoped Γ Γ' η -> subscoped Γ Γ' (substcomp ξ η).
 Proof.
 (*   intros. intro. intros. unfold substcomp. break_match_goal;
   [ apply H | apply H0 ]; auto. *)
   
-Abort.
+Abort. *)
 
 Lemma subst_list_in_val : forall l x vals ξ, length l = length vals ->
   In x l -> exists v, In v vals /\ (ξ[[ ::= combine l vals]]) x = v.
@@ -214,7 +263,7 @@ Proof.
       unfold extend_subst. rewrite var_funid_eqb_refl. auto.
 Qed.
 
-Lemma subscoped_ext_app :
+(* Lemma subscoped_ext_app :
   forall ξ Γ Γ' l vals, subscoped Γ Γ' ξ -> length l = length vals ->
   Forall (fun v => VAL Γ' ⊢ v ) vals ->
   subscoped (Γ ++ l) Γ' (substcomp (idsubst[[::= combine l vals]]) (ξ -- l)).
@@ -224,7 +273,7 @@ Proof.
     - apply in_list_sound in Heqb. Check subst_list_in.
       epose (subst_list_in_val _ _ _ _ H0 Heqb). destruct e. destruct H3.
       rewrite H4. rewrite indexed_to_forall in H1. (* Just technical, but doable *) *)
-Admitted.
+Admitted. *)
 
 Lemma biforall_vrel_helper : forall m vals1 vals2, length vals1 = length vals2 ->
   list_biforall (Vrel m) vals1 vals2 ->
@@ -240,6 +289,28 @@ Proof.
     - apply (IHvals1 x0); auto.
 Qed.
 
+(* Lemma alma :
+  forall e ξ x v, 
+                  subst (idsubst[[x ::= v]]) (subst (ξ -- [x]) e) =
+                  subst (ξ[[x ::= v]]) e.
+Proof.
+  induction e; intros; subst; try reflexivity.
+  * unfold "--", extend_subst. cbn. break_match_goal.
+    - break_match_goal.
+      + apply var_funid_eqb_eq in Heqb0. subst. cbn. rewrite eqb_refl. auto.
+      + apply var_funid_eqb_neq in Heqb0. break_match_hyp.
+        ** destruct x.
+           -- apply eqb_eq in Heqb1. subst. contradiction.
+           -- congruence.
+        ** congruence.
+    - break_match_goal.
+      + apply var_funid_eqb_eq in Heqb0. subst. rewrite eqb_refl in Heqb. congruence.
+      + break_match_hyp.
+        ** congruence.
+        ** destruct x.
+           -- apply 
+Qed. *)
+
 Lemma Vrel_Fun_compat :
   forall Γ vl b1 b2,
   Erel_open (Γ ++ map inl vl) b1 b2 ->
@@ -248,9 +319,9 @@ Proof.
   intros. unfold Vrel_open. intros.
   inversion H0 as [? [? ?] ].
   simpl. rewrite Vrel_Fix_eq. unfold Vrel_rec at 1. intuition idtac.
-  - constructor. eapply subst_preserves_scope_rev; eauto. eapply Erel_open_scope in H. apply H.
-  - constructor. eapply subst_preserves_scope_rev; eauto. eapply Erel_open_scope in H. apply H.
-  - break_match_goal; try congruence. intros. unfold Erel_open in H.
+  - constructor. eapply subst_preserves_scope_rev; eauto.
+  - constructor. eapply subst_preserves_scope_rev; eauto.
+  - break_match_goal; try congruence. intros. unfold Erel_open, Erel in H.
     Search subst.
 (*     rewrite subst_composition; eauto.
     unfold Erel in H.
@@ -279,14 +350,30 @@ Proof.
   unfold Erel, exp_rel.
   pose proof (Vrel_possibilities H).
   intuition eauto.
-  apply Vrel_closed in H; destruct H.
-  1-2: try destruct H1, H0; subst; repeat try constructor.
+  1-2, 4, 5, 7, 8: apply Vrel_closed in H; destruct H.
+  1-7: repeat try constructor; auto.
   destruct H1, H1; subst. destruct m; inversion H0. subst.
   eexists. split. exists 1. reflexivity. eapply Vrel_downclosed. eauto.
-  1-2: try destruct H0, H0, H0, H0, H0; subst; repeat try constructor.
+  destruct H0, H0, H0, H0, H0. subst. destruct m; inversion H1. subst.
+  eexists. split. exists 1. reflexivity. eapply Vrel_downclosed. eauto.
+  destruct H0, H0, H0, H0, H0, H0, H0. subst. destruct m; inversion H1. subst.
+  eexists. split. exists 1. reflexivity. eapply Vrel_downclosed. eauto.
+Unshelve. all: auto.
 Qed.
 
 Hint Resolve Erel_Val_compatible_closed.
+
+Lemma Erel_Val_compatible :
+  forall {Γ v v'},
+    Vrel_open Γ v v' ->
+    Erel_open Γ v v'.
+Proof.
+  intros.
+  unfold Erel_open, Vrel_open in *.
+  auto.
+Qed.
+
+Hint Resolve Erel_Val_compatible.
 
 (*
 Lemma Expr_cons :
@@ -310,18 +397,6 @@ Proof.
 Qed.
 
 Hint Resolve Expr_cons.
-
-Lemma Erel_Val_compatible :
-  forall {Γ v v'},
-    Vrel_open Γ v v' ->
-    Erel_open Γ v v'.
-Proof.
-  intros.
-  unfold Erel_open, Vrel_open in *.
-  auto.
-Qed.
-
-Hint Resolve Erel_Val_compatible.
 
 Lemma Erel_Var_compatible :
   forall Γ x,
